# completing the square
i cant really imagine not understanding this but just in case heres a thing

## but first, a message from basic factoring
so if you evaluated $(x+y)^2$ you'd notice that it's equal to $x^2+2xy+y^2$.

now if you have a quadratic equation like

$$x^2+6x+9=1$$

then you can do

$$\begin{aligned}x^2+6x+9 &= 0 \\ x^2+2(3x)+3^2 &= 0 \\ (x+3)^2 &= 0 \\ x+3 &= 0 \\ x &= -3 \end{aligned}$$

## actual stuff

ok now heres another

$$x^2 + 6x + 8 = 0$$

now we can't do what we did earlier

except that we totally can:

$$\begin{aligned}
x^2+6x &= -8 \\
x^2+6x+9 &= -8+9 \text{ (!) great move ;)}\\
x^2+6x+3^2 &= 1 \\
&=(x+3)^2 \\
x+3 &= \pm1 \\
x_1 &= 1-3 \\
&= -2 \\
x_2 &= -1-3 \\
&= -4
\end{aligned}$$

(you could also factor but shut up)

so yeah if you just did that you just completed a square gj

## cool shit you can do
 * [quadratic formula](../formula)
 * <sup><sub>make fun of innocent kid sitting next to you for not understanding factoring then come first in the school ahead of 12th graders in big math contest (not based on a true story)</sub></sup>
